models/oalts/Tree.v
@@ -8,13 +8,14 @@ Module Tree. (* <: Category. *)
   Import AsyncEvents.
 
   Variant treeF (A : Type) (tree : Type) : Type :=
-  (* step *)
-  | StepF {X : Type} (step : X -> A) (k : X -> tree).
+  | StepF (X : Type) (step : X -> A) (k : X -> tree)
+  | EpsF (k : tree).
 
   CoInductive tree (A : Type) : Type :=
     go { _observe : treeF A (tree A) }.
 
-  Arguments StepF {A} [tree] [X].
+  Arguments StepF {A} [tree].
+  Arguments EpsF {A} [tree].
   Arguments _observe {A}.
   Arguments go {A}.
 
@@ -24,173 +25,191 @@ Module Tree. (* <: Category. *)
 
   Lemma tree_eta : forall {A} (t : tree A), t = go (observe t).
   Proof.
-    intros A t. destruct t as [[X step k]]. reflexivity.
+    intros A t. destruct t; reflexivity.
   Qed.
 
-  Section Simulation.
-    Definition simF {A : Type}
+  Section StrongSimulation.
+    Definition ssimF {A : Type}
       (R : tree A -> tree A -> Prop) (p : tree A) (q : tree A) : Prop :=
       match observe p, observe q with
-      |  @StepF _ _ X step_p k_p, @StepF _ _ X' step_q k_q =>
+      |  StepF X step_p k_p, StepF X' step_q k_q =>
         forall x, exists x', step_p x = step_q x' /\ R (k_p x) (k_q x')
+      | EpsF p', EpsF q' => R p' q'
+      | _, _ => False
       end.
 
-    Lemma simF_mon {A : Type} : monotone2 (@simF A).
+    Lemma ssimF_mon {A : Type} : monotone2 (@ssimF A).
     Proof.
-      unfold monotone2, simF. intros p q R R' H LE.
-      destruct (observe p) as [X step_p k_p].
-      destruct (observe q) as [X' step_q k_q].
+      unfold monotone2, ssimF. intros p q R R' H LE.
+      destruct (observe p) as [X step_p k_p | p'];
+      destruct (observe q) as [X' step_q k_q | q'];
+      try apply LE; try assumption.
       intros x. specialize (H x).
       destruct H as [x' [Heq HR]]. exists x'. split; auto.
     Qed.
 
-    Hint Resolve simF_mon : paco.
+    Hint Resolve ssimF_mon : paco.
 
-    Lemma simF_refl {A : Type} (R : tree A -> tree A -> Prop) (p : tree A) :
-      (forall t, R t t) -> simF R p p.
+    Lemma ssimF_refl {A : Type} (R : tree A -> tree A -> Prop) (p : tree A) :
+      (forall t, R t t) -> ssimF R p p.
     Proof.
-      unfold simF. intros Hrefl.
-      destruct (observe p) as [X step_p k_p].
-      intros x. exists x. split.
-      - reflexivity.
+      unfold ssimF. intros Hrefl.
+      destruct (observe p) as [X step_p k_p | p'].
+      - intros x. exists x. split.
+        + reflexivity.
+        + apply Hrefl.
       - apply Hrefl.
     Qed.
 
-    Lemma simF_trans {A : Type} (R S : tree A -> tree A -> Prop) (p q s : tree A) :
-      simF R p q -> simF S q s -> simF (rel_compose R S) p s.
+    Lemma ssimF_trans {A : Type} (R S : tree A -> tree A -> Prop) (p q s : tree A) :
+      ssimF R p q -> ssimF S q s -> ssimF (rel_compose R S) p s.
     Proof.
-      unfold simF. intros Hpq Hqs.
-      destruct (observe p) as [X step_p k_p].
-      destruct (observe q) as [Y step_q k_q].
-      destruct (observe s) as [Z step_s k_s].
-      intros x.
-      specialize (Hpq x). destruct Hpq as [y [Heq_pq HR_pq]].
-      specialize (Hqs y). destruct Hqs as [z [Heq_qs HR_qs]].
-      exists z. split.
-      - transitivity (step_q y); assumption.
-      - exists (k_q y). split; assumption.
+      unfold ssimF. intros Hpq Hqs.
+      destruct (observe p) as [X step_p k_p | p'];
+      destruct (observe q) as [Y step_q k_q | q'];
+      destruct (observe s) as [Z step_s k_s | s'];
+      try contradiction.
+      - intros x.
+        specialize (Hpq x). destruct Hpq as [y [Heq_pq HR_pq]].
+        specialize (Hqs y). destruct Hqs as [z [Heq_qs HR_qs]].
+        exists z. split.
+        + transitivity (step_q y); assumption.
+        + exists (k_q y). split; assumption.
+      - exists q'. split; assumption.
     Qed.
 
-    Definition sim {A : Type} : tree A -> tree A -> Prop :=
-      paco2 simF bot2.
+    Definition ssim {A : Type} : tree A -> tree A -> Prop :=
+      paco2 ssimF bot2.
 
-    Proposition simF_sim : forall {A : Type} (p : tree A) (q : tree A),
-      simF (sim) p q -> sim p q.
+    Proposition ssimF_ssim : forall {A : Type} (p : tree A) (q : tree A),
+      ssimF (ssim) p q -> ssim p q.
     Proof.
-      intros A p q H. pfold. unfold simF in *.
-      destruct (observe p) as [X step_p k_p].
-      destruct (observe q) as [X' step_q k_q].
-      intros x. specialize (H x).
-      destruct H as [x' [Heq HR]]. exists x'. split; auto.
+      intros A p q H. pfold. unfold ssimF in *.
+      destruct (observe p) as [X step_p k_p | p'];
+      destruct (observe q) as [X' step_q k_q | q'];
+      try assumption.
+      - intros x. specialize (H x).
+        destruct H as [x' [Heq HR]]. exists x'. split; auto.
+      - left. exact H.
     Qed.
 
-    Proposition sim_simF : forall {A : Type} (p : tree A) (q : tree A),
-      sim p q -> simF sim p q.
+    Proposition ssim_ssimF : forall {A : Type} (p : tree A) (q : tree A),
+      ssim p q -> ssimF ssim p q.
     Proof.
-      intros A p q H. punfold H. unfold simF in *.
-      destruct (observe p) as [X step_p k_p].
-      destruct (observe q) as [X' step_q k_q].
-      intros x. specialize (H x).
-      destruct H as [x' [Heq HR]]. exists x'. split; auto.
-      destruct HR; auto. contradiction.
+      intros A p q H. punfold H. unfold ssimF in *.
+      destruct (observe p) as [X step_p k_p | p'];
+      destruct (observe q) as [X' step_q k_q | q'];
+      try assumption.
+      - intros x. specialize (H x).
+        destruct H as [x' [Heq HR]]. exists x'. split; auto.
+        destruct HR; auto. contradiction.
+      - destruct H; auto. contradiction.
     Qed.
 
-    Proposition sim_refl {A : Type} (p : tree A) : sim p p.
+    Proposition ssim_refl {A : Type} (p : tree A) : ssim p p.
     Proof.
       revert p. pcofix IH. intros p. pfold.
-      apply simF_refl. intros t. right. apply IH.
+      apply ssimF_refl. intros t. right. apply IH.
     Qed.
 
-    Proposition sim_trans {A : Type} (p q s : tree A) :
-      sim p q -> sim q s -> sim p s.
+    Proposition ssim_trans {A : Type} (p q s : tree A) :
+      ssim p q -> ssim q s -> ssim p s.
     Proof.
       revert p q s. pcofix IH. intros p q s Hpq Hqs.
       punfold Hpq. punfold Hqs. pfold.
-      eapply simF_mon.
-      - eapply simF_trans; eassumption.
+      eapply ssimF_mon.
+      - eapply ssimF_trans; eassumption.
       - intros a c [b [Hab Hbc]].
         destruct Hab as [Hab | []]. destruct Hbc as [Hbc | []].
         right. eapply IH; eassumption.
     Qed.
-  End Simulation.
+  End StrongSimulation.
 
-  #[export] Hint Resolve simF_mon : paco.
+  #[export] Hint Resolve ssimF_mon : paco.
 
-  Section Bisimulation.
-    Definition bisimF {A : Type}
+  Section StrongBisimulation.
+    Definition sbisimF {A : Type}
       (R : tree A -> tree A -> Prop) (p : tree A) (q : tree A) : Prop :=
       match observe p, observe q with
-      |  @StepF _ _ X step_p k_p, @StepF _ _ X' step_q k_q =>
+      | StepF X step_p k_p, StepF X' step_q k_q =>
         (forall x, exists x', step_p x = step_q x' /\ R (k_p x) (k_q x')) /\
         (forall x', exists x, step_p x = step_q x' /\ R (k_p x) (k_q x'))
+      | EpsF p', EpsF q' => R p' q'
+      | _, _ => False
       end.
 
-    Lemma bisimF_mon {A : Type} : monotone2 (@bisimF A).
+    Lemma sbisimF_mon {A : Type} : monotone2 (@sbisimF A).
     Proof.
-      unfold monotone2, bisimF. intros p q R R' H LE.
-      destruct (observe p) as [X step_p k_p].
-      destruct (observe q) as [X' step_q k_q].
+      unfold monotone2, sbisimF. intros p q R R' H LE.
+      destruct (observe p) as [X step_p k_p | p'];
+      destruct (observe q) as [X' step_q k_q | q'];
+      try apply LE; try assumption.
       destruct H as [Hfw Hbw]; split.
       - intros x. specialize (Hfw x).
         destruct Hfw as [x' [Heq Hr]].
-        exists x'. split. 2: apply LE. 
-        all: assumption. 
+        exists x'. split. 2: apply LE.
+        all: assumption.
       - intros x'. specialize (Hbw x').
         destruct Hbw as [x [Heq Hr]].
-        exists x. split. 2: apply LE. 
+        exists x. split. 2: apply LE.
         all: assumption.
     Qed.
 
-    Hint Resolve bisimF_mon : paco.
+    Hint Resolve sbisimF_mon : paco.
 
-    Lemma bisimF_refl {A : Type} (R : tree A -> tree A -> Prop) (p : tree A) :
-      (forall t, R t t) -> bisimF R p p.
+    Lemma sbisimF_refl {A : Type} (R : tree A -> tree A -> Prop) (p : tree A) :
+      (forall t, R t t) -> sbisimF R p p.
     Proof.
-      unfold bisimF. intros Hrefl.
-      destruct (observe p) as [X step_p k_p].
-      split; intros x; exists x; split; 
-      try reflexivity; try (apply Hrefl).
+      unfold sbisimF. intros Hrefl.
+      destruct (observe p) as [X step_p k_p | p'].
+      - split; intros x; exists x; split;
+        try reflexivity; try (apply Hrefl).
+      - apply Hrefl.
     Qed.
 
-    Lemma bisimF_trans {A : Type} (R S : tree A -> tree A -> Prop) (p q s : tree A) :
-      bisimF R p q -> bisimF S q s -> bisimF (rel_compose R S) p s.
+    Lemma sbisimF_trans {A : Type} (R S : tree A -> tree A -> Prop) (p q s : tree A) :
+      sbisimF R p q -> sbisimF S q s -> sbisimF (rel_compose R S) p s.
     Proof.
-      unfold bisimF. intros Hpq Hqs.
-      destruct (observe p) as [X step_p k_p].
-      destruct (observe q) as [Y step_q k_q].
-      destruct (observe s) as [Z step_s k_s].
-      destruct Hpq as [Hpq_fw Hpq_bw].
-      destruct Hqs as [Hqs_fw Hqs_bw].
-      split.
-      - intros x.
-        specialize (Hpq_fw x). destruct Hpq_fw as [y [Heq_pq HR_pq]].
-        specialize (Hqs_fw y). destruct Hqs_fw as [z [Heq_qs HR_qs]].
-        exists z. split.
-        + transitivity (step_q y); assumption.
-        + exists (k_q y). split; assumption.
-      - intros z.
-        specialize (Hqs_bw z). destruct Hqs_bw as [y [Heq_qs HR_qs]].
-        specialize (Hpq_bw y). destruct Hpq_bw as [x [Heq_pq HR_pq]].
-        exists x. split.
-        + transitivity (step_q y); assumption.
-        + exists (k_q y). split; assumption.
+      unfold sbisimF. intros Hpq Hqs.
+      destruct (observe p) as [X step_p k_p | p'];
+      destruct (observe q) as [Y step_q k_q | q'];
+      destruct (observe s) as [Z step_s k_s | s'];
+      try contradiction.
+      - destruct Hpq as [Hpq_fw Hpq_bw].
+        destruct Hqs as [Hqs_fw Hqs_bw].
+        split.
+        + intros x.
+          specialize (Hpq_fw x). destruct Hpq_fw as [y [Heq_pq HR_pq]].
+          specialize (Hqs_fw y). destruct Hqs_fw as [z [Heq_qs HR_qs]].
+          exists z. split.
+          * transitivity (step_q y); assumption.
+          * exists (k_q y). split; assumption.
+        + intros z.
+          specialize (Hqs_bw z). destruct Hqs_bw as [y [Heq_qs HR_qs]].
+          specialize (Hpq_bw y). destruct Hpq_bw as [x [Heq_pq HR_pq]].
+          exists x. split.
+          * transitivity (step_q y); assumption.
+          * exists (k_q y). split; assumption.
+      - exists q'. split; assumption.
     Qed.
 
-    Lemma bisimF_simF {A : Type} (R : tree A -> tree A -> Prop) (p q : tree A) :
-      bisimF R p q -> simF R p q.
+    Lemma sbisimF_ssimF {A : Type} (R : tree A -> tree A -> Prop) (p q : tree A) :
+      sbisimF R p q -> ssimF R p q.
     Proof.
-      unfold bisimF, simF.
-      destruct (observe p) as [X step_p k_p].
-      destruct (observe q) as [X' step_q k_q].
+      unfold sbisimF, ssimF.
+      destruct (observe p) as [X step_p k_p | p'];
+      destruct (observe q) as [X' step_q k_q | q'];
+      try contradiction; auto.
       intros [Hfw _]. exact Hfw.
     Qed.
 
-    Proposition bisimF_sym {A : Type} (R : tree A -> tree A -> Prop) (p q : tree A) :
-      bisimF R p q -> bisimF (flip R) q p.
+    Proposition sbisimF_sym {A : Type} (R : tree A -> tree A -> Prop) (p q : tree A) :
+      sbisimF R p q -> sbisimF (flip R) q p.
     Proof.
-      unfold bisimF.
-      destruct (observe p) as [X step_p k_p].
-      destruct (observe q) as [X' step_q k_q].
+      unfold sbisimF.
+      destruct (observe p) as [X step_p k_p | p'];
+      destruct (observe q) as [X' step_q k_q | q'];
+      try contradiction; auto.
       intros [Hfw Hbw]. split.
       - intros x'. specialize (Hbw x').
         destruct Hbw as [x [Heq HR]].
@@ -204,106 +223,114 @@ Module Tree. (* <: Category. *)
         + exact HR.
     Qed.
 
-    Lemma bisimF_mutual_simF {A : Type} (R : tree A -> tree A -> Prop) (p q : tree A) :
-      bisimF R p q <-> simF R p q /\ simF (flip R) q p.
+    Lemma sbisimF_mutual_ssimF {A : Type} (R : tree A -> tree A -> Prop) (p q : tree A) :
+      sbisimF R p q <-> ssimF R p q /\ ssimF (flip R) q p.
     Proof.
       split.
       - intros H. split.
-        + apply bisimF_simF. exact H.
-        + apply bisimF_simF. apply bisimF_sym. exact H.
-      - unfold bisimF, simF.
-        destruct (observe p) as [X step_p k_p].
-        destruct (observe q) as [X' step_q k_q].
-        intros [Hfw Hbw]. split.
-        + exact Hfw.
+        + apply sbisimF_ssimF. exact H.
+        + apply sbisimF_ssimF. apply sbisimF_sym. exact H.
+      - unfold sbisimF, ssimF.
+        destruct (observe p) as [X step_p k_p | p'];
+        destruct (observe q) as [X' step_q k_q | q'].
+        + intros [Hfw Hbw]. split.
+          * exact Hfw.
+          * intros x'. specialize (Hbw x').
+            destruct Hbw as [x [Heq HR]].
+            exists x. split.
+            -- symmetry. exact Heq.
+            -- exact HR.
+        + intros [Hfw _]. contradiction.
+        + intros [Hfw _]. contradiction.
+        + intros [Hfw _]. exact Hfw.
+    Qed.
+
+    Definition sbisim {A : Type} : tree A -> tree A -> Prop :=
+      paco2 (sbisimF) bot2.
+
+    Proposition sbisimF_sbisim : forall {A : Type} (p : tree A) (q : tree A),
+      sbisimF sbisim p q -> sbisim p q.
+    Proof.
+      intros A p q H. pfold. unfold sbisimF in *.
+      destruct (observe p) as [X step_p k_p | p'];
+      destruct (observe q) as [X' step_q k_q | q'];
+      try assumption.
+      - destruct H as [Hfw Hbw]. split.
+        + intros x. specialize (Hfw x).
+          destruct Hfw as [x' [Heq HR]]. exists x'. split; auto.
         + intros x'. specialize (Hbw x').
-          destruct Hbw as [x [Heq HR]].
-          exists x. split.
-          * symmetry. exact Heq.
-          * exact HR.
+          destruct Hbw as [x [Heq HR]]. exists x. split; auto.
+      - left. exact H.
     Qed.
 
-    Definition bisim {A : Type} : tree A -> tree A -> Prop :=
-      paco2 (bisimF) bot2.
-
-    Proposition bisimF_bisim : forall {A : Type} (p : tree A) (q : tree A),
-      bisimF bisim p q -> bisim p q.
+    Proposition sbisim_sbisimF : forall {A : Type} (p : tree A) (q : tree A),
+      sbisim p q -> sbisimF sbisim p q.
     Proof.
-      intros A p q H. pfold. unfold bisimF in *.
-      destruct (observe p) as [X step_p k_p].
-      destruct (observe q) as [X' step_q k_q].
-      destruct H as [Hfw Hbw]. split.
-      - intros x. specialize (Hfw x).
-        destruct Hfw as [x' [Heq HR]]. exists x'. split; auto.
-      - intros x'. specialize (Hbw x').
-        destruct Hbw as [x [Heq HR]]. exists x. split; auto.
+      intros A p q H. punfold H. unfold sbisimF in *.
+      destruct (observe p) as [X step_p k_p | p'];
+      destruct (observe q) as [X' step_q k_q | q'];
+      try assumption.
+      - destruct H as [Hfw Hbw]. split.
+        + intros x. specialize (Hfw x).
+          destruct Hfw as [x' [Heq HR]]. exists x'. split; auto.
+          destruct HR; auto. contradiction.
+        + intros x'. specialize (Hbw x').
+          destruct Hbw as [x [Heq HR]]. exists x. split; auto.
+          destruct HR; auto. contradiction.
+      - destruct H; auto. contradiction.
     Qed.
 
-    Proposition bisim_bisimF : forall {A : Type} (p : tree A) (q : tree A),
-      bisim p q -> bisimF bisim p q.
-    Proof.
-      intros A p q H. punfold H. unfold bisimF in *.
-      destruct (observe p) as [X step_p k_p].
-      destruct (observe q) as [X' step_q k_q].
-      destruct H as [Hfw Hbw]. split.
-      - intros x. specialize (Hfw x).
-        destruct Hfw as [x' [Heq HR]]. exists x'. split; auto.
-        destruct HR; auto. contradiction.
-      - intros x'. specialize (Hbw x').
-        destruct Hbw as [x [Heq HR]]. exists x. split; auto.
-        destruct HR; auto. contradiction.
-    Qed.
-
-    Proposition bisim_refl {A : Type} (p : tree A) : bisim p p.
+    Proposition sbisim_refl {A : Type} (p : tree A) : sbisim p p.
     Proof.
       revert p. pcofix IH. intros p. pfold.
-      apply bisimF_refl. intros t. right. apply IH.
+      apply sbisimF_refl. intros t. right. apply IH.
     Qed.
 
-    Proposition bisim_sym {A : Type} (p q : tree A) : bisim p q -> bisim q p.
+    Proposition sbisim_sym {A : Type} (p q : tree A) : sbisim p q -> sbisim q p.
     Proof.
       revert p q. pcofix IH. intros p q H.
       punfold H. pfold.
-      apply bisimF_sym in H.
-      eapply bisimF_mon. exact H.
+      apply sbisimF_sym in H.
+      eapply sbisimF_mon. exact H.
       intros p' q' Hflip. unfold flip in Hflip.
       destruct Hflip as [Hflip | []].
       right. apply IH. exact Hflip.
     Qed.
 
-    Proposition bisim_trans {A : Type} (p q s : tree A) :
-      bisim p q -> bisim q s -> bisim p s.
+    Proposition sbisim_trans {A : Type} (p q s : tree A) :
+      sbisim p q -> sbisim q s -> sbisim p s.
     Proof.
       revert p q s. pcofix IH. intros p q s Hpq Hqs.
       punfold Hpq. punfold Hqs. pfold.
-      eapply bisimF_mon.
-      - eapply bisimF_trans; eassumption.
+      eapply sbisimF_mon.
+      - eapply sbisimF_trans; eassumption.
       - intros a c [b [Hab Hbc]].
         destruct Hab as [Hab | []]. destruct Hbc as [Hbc | []].
         right. eapply IH; eassumption.
     Qed.
 
-    Lemma bisim_sim_fwd {A : Type} (p q : tree A) :
-      bisim p q -> sim p q.
+    Lemma sbisim_ssim_fwd {A : Type} (p q : tree A) :
+      sbisim p q -> ssim p q.
     Proof.
       revert p q. pcofix IH. intros p q H.
       punfold H. pfold.
-      apply bisimF_simF in H.
-      eapply simF_mon. exact H.
+      apply sbisimF_ssimF in H.
+      eapply ssimF_mon. exact H.
       intros p' q' Hbisim.
       destruct Hbisim as [Hbisim | []].
       right. apply IH. exact Hbisim.
     Qed.
 
-    Proposition bisim_impl_sim {A : Type} (p q : tree A) :
-      bisim p q -> sim p q /\ sim q p.
+    Proposition sbisim_impl_ssim {A : Type} (p q : tree A) :
+      sbisim p q -> ssim p q /\ ssim q p.
     Proof.
       intros H. split.
-      - apply bisim_sim_fwd. exact H.
-      - apply bisim_sim_fwd. apply bisim_sym. exact H.
+      - apply sbisim_ssim_fwd. exact H.
+      - apply sbisim_ssim_fwd. apply sbisim_sym. exact H.
     Qed.
 
-  End Bisimulation.
+  End StrongBisimulation.
+
+  #[export] Hint Resolve sbisimF_mon : paco.
 
 End Tree.
-
